add const entries { } to the P4 program. So currently the P4 program is not the same as compiled by the Tofino compiler, but it's because Tofino compiler is not up to date with the P4 spec

examples/sbf/verif_Filter.v
@@ -108,14 +108,20 @@ Definition tbl_hash_index_1_spec : func_spec :=
         (MEM [(["ds_key"], eval_val_to_sval key); (["ds_md"], ds_md)]
         (EXT [])))
       POST
-        (ARG_RET [] ValBaseNull
+        (EX retv,
+        (ARG_RET [] retv
         (MEM [(["ds_md"], update "hash_index_1" (P4Bit 18 (hash1 key)) ds_md)]
-        (EXT []))).
+        (EXT []))))%arg_ret_assr.
 
 Lemma tbl_hash_index_1_body :
   func_sound ge tbl_hash_index_1_fd nil tbl_hash_index_1_spec.
 Proof.
-Admitted.
+  start_function.
+  next_case.
+  table_action act_hash_index_1_body.
+  { entailer. }
+  { entailer. }
+Qed.
 
 #[local] Hint Extern 5 (func_modifies _ _ _ _ _) => (apply tbl_hash_index_1_body) : func_specs.
 
@@ -169,13 +175,35 @@ Proof.
   entailer.
 Qed.
 
+#[local] Hint Extern 5 (func_modifies _ _ _ _ _) => (apply act_hash_index_2_body) : func_specs.
+
 Definition tbl_hash_index_2_fd :=
   ltac:(get_fd ["Bf2BloomFilter"; "tbl_hash_index_2"; "apply"] ge).
 
+Definition tbl_hash_index_2_spec : func_spec :=
+  WITH (* p *),
+    PATH p
+    MOD (Some [["ds_md"]; ["act_hash_index_2"; "t'1"]]) []
+    WITH (key : Val) (ds_md : Sval),
+      PRE
+        (ARG []
+        (MEM [(["ds_key"], eval_val_to_sval key); (["ds_md"], ds_md)]
+        (EXT [])))
+      POST
+        (EX retv,
+        (ARG_RET [] retv
+        (MEM [(["ds_md"], update "hash_index_2" (P4Bit 18 (hash2 key)) ds_md)]
+        (EXT []))))%arg_ret_assr.
+
 Lemma tbl_hash_index_2_body :
-  func_sound ge tbl_hash_index_2_fd nil act_hash_index_2_spec.
+  func_sound ge tbl_hash_index_2_fd nil tbl_hash_index_2_spec.
 Proof.
-Admitted.
+  start_function.
+  next_case.
+  table_action act_hash_index_2_body.
+  { entailer. }
+  { entailer. }
+Qed.
 
 #[local] Hint Extern 5 (func_modifies _ _ _ _ _) => (apply tbl_hash_index_2_body) : func_specs.
 
@@ -229,13 +257,35 @@ Proof.
   entailer.
 Qed.
 
+#[local] Hint Extern 5 (func_modifies _ _ _ _ _) => (apply act_hash_index_3_body) : func_specs.
+
 Definition tbl_hash_index_3_fd :=
   ltac:(get_fd ["Bf2BloomFilter"; "tbl_hash_index_3"; "apply"] ge).
 
+Definition tbl_hash_index_3_spec : func_spec :=
+  WITH (* p *),
+    PATH p
+    MOD (Some [["ds_md"]; ["act_hash_index_3"; "t'2"]]) []
+    WITH (key : Val) (ds_md : Sval),
+      PRE
+        (ARG []
+        (MEM [(["ds_key"], eval_val_to_sval key); (["ds_md"], ds_md)]
+        (EXT [])))
+      POST
+        (EX retv,
+        (ARG_RET [] retv
+        (MEM [(["ds_md"], update "hash_index_3" (P4Bit 18 (hash3 key)) ds_md)]
+        (EXT []))))%arg_ret_assr.
+
 Lemma tbl_hash_index_3_body :
-  func_sound ge tbl_hash_index_3_fd nil act_hash_index_3_spec.
+  func_sound ge tbl_hash_index_3_fd nil tbl_hash_index_3_spec.
 Proof.
-Admitted.
+  start_function.
+  next_case.
+  table_action act_hash_index_3_body.
+  { entailer. }
+  { entailer. }
+Qed.
 
 #[local] Hint Extern 5 (func_modifies _ _ _ _ _) => (apply tbl_hash_index_3_body) : func_specs.
 
@@ -329,13 +379,35 @@ Proof.
   }
 Qed.
 
+#[local] Hint Extern 5 (func_modifies _ _ _ _ _) => (apply act_clear_index_body) : func_specs.
+
 Definition tbl_clear_index_fd :=
   ltac:(get_fd ["Bf2BloomFilter"; "tbl_clear_index"; "apply"] ge).
 
+Definition tbl_clear_index_spec : func_spec :=
+  WITH (* p *),
+    PATH p
+    MOD (Some [["ds_md"]; ["act_clear_index"; "t'3"]]) [p ++ ["reg_clear_index"]]
+    WITH (i : Z) (ds_md : Sval),
+      PRE
+        (ARG []
+        (MEM [(["ds_md"], ds_md)]
+        (EXT [fil_clear_index_repr p 18 i])))
+      POST
+        (EX retv,
+        (ARG_RET [] retv
+        (MEM [(["ds_md"], update "clear_index_1" (P4Bit 18 i) ds_md)]
+        (EXT [fil_clear_index_repr p 18 (update_clear_index (num_slots := num_slots) i)]))))%arg_ret_assr.
+
 Lemma tbl_clear_index_body :
-  func_sound ge tbl_clear_index_fd nil act_clear_index_spec.
+  func_sound ge tbl_clear_index_fd nil tbl_clear_index_spec.
 Proof.
-Admitted.
+  start_function.
+  next_case.
+  table_action act_clear_index_body.
+  { entailer. }
+  { entailer. }
+Qed.
 
 #[local] Hint Extern 5 (func_modifies _ _ _ _ _) => (apply tbl_clear_index_body) : func_specs.
 
@@ -1715,12 +1787,15 @@ Proof.
   Time step_call tbl_hash_index_1_body.
   { entailer. }
   Time simpl_assertion.
+  Intros _.
   step_call tbl_hash_index_2_body.
   { entailer. }
   Time simpl_assertion.
+  Intros _.
   step_call tbl_hash_index_3_body.
   { entailer. }
   Time simpl_assertion.
+  Intros _.
   set (is := (exist _ [hash1 key; hash2 key; hash3 key] eq_refl : listn Z 3)).
   set (clear_is := (exist _ (Zrepeat fil_clear_index 3) eq_refl : listn Z 3)).
   assert (Forall (fun i : Z => 0 <= i < num_slots) (`is)). {
@@ -1740,6 +1815,7 @@ Proof.
   step_call tbl_clear_index_body.
   { entailer. }
   Time simpl_assertion.
+  Intros _.
   step_call tbl_clear_window_body.
   { entailer. }
   Intros _.
